

# Floating-point numbers in Ginger

November 6, 2012

In this section I shall describe a new way to represent floating point numbers in Ginger. We consider  $m \times m$  matrix multiplication and require the input entries in the set  $T = \{a/b : |a| \leq 2^{N_a}, b \in \{1, 2, 2^2, 2^3, \dots, 2^{N_b}\}\}$ . Previously, it was shown that  $p > (m+1)^2 \cdot 2^{4(N_a+N_b)}$  is necessary for making  $\theta$  1-1 which is required to make the mapping isomorphic from  $U$  to  $\mathbb{Q}/p$ . In this exercise I show that by modifying the definition of  $\theta$  and the mapped field, one can obtain a better bound on  $p$  (i.e.,  $p > \max\{2m \cdot 2^{2N_a+2N_b}, 2N_a + 4N_b + \log_2 m\}$ ). I do not make any changes to step C1. The changes I propose, with the resulting proofs are described below:

Define  $\theta$  as follows:

$$\theta : U \rightarrow \mathbb{F}$$

$$\frac{a}{b = 2^k} \mapsto (a \bmod p, k \bmod p)$$

The field  $\mathbb{F}$  is the set of equivalence classes on the set  $\mathbb{Z}/p \times \mathbb{Z}/p$  under the equivalence relation:  $(a, b) \sim (c, d)$  if  $\ell \equiv s \pmod{p}$  and  $r_1 + d \equiv r_2 + b \pmod{p}$ , where  $a = \ell \cdot 2^{r_1}$  and  $c = s \cdot 2^{r_2}$ . We have written  $a$  and  $c$  in this form by factoring out all the powers of 2. Every integer can be written in this form (for integer greater than 1 this follows from fundamental theorem of arithmetic, and  $1 = 1 \cdot 2^0$  and  $0 = 0 \cdot 2^k$  where  $k$  is arbitrary).

The addition operation is defined by  $(a, b) + (c, d) = (a \cdot 2^d + c \cdot 2^b, b + d)$

The multiplication operation is defined by  $(a, b) \cdot (c, d) = (a \cdot c, b + d)$

$(1, 0)$  is the multiplicative identity. For any  $(a, b) \in \mathbb{F}$  (except additive identity of course)  $(a^{-1}, -b)$  is the multiplicative inverse.  $(0, 0)$  is the additive identity (in fact  $(0, 0) \sim (0, k)$ ). For any  $(a, b) \in \mathbb{F}$ ,  $(-a, b)$  is the additive inverse. Now we show that  $\theta$  preserves addition and multiplication rules for  $q_1, q_2 \in U$ .

$$\theta(q_1 + q_2) = \theta\left(\frac{a_1}{b_1} + \frac{a_2}{b_2}\right) = \theta\left(\frac{a_1 \cdot b_2 + a_2 \cdot b_1}{2^{k_1} \cdot 2^{k_2}}\right) = (a_1 \cdot b_2 + a_2 \cdot b_1, k_1 + k_2)$$

$$\theta(q_1) + \theta(q_2) = (a_1, k_1) + (a_2, k_2) = (a_1 \cdot 2^{k_2} + a_2 \cdot 2^{k_1}, k_1 + k_2)$$

$$\text{so, } \theta(q_1 + q_2) = \theta(q_1) + \theta(q_2)$$

Similarly, the multiplication rule holds:

$$\theta(q_1 \cdot q_2) = \theta\left(\frac{a_1 \cdot a_2}{b_1 \cdot b_2}\right) = \theta\left(\frac{a_1 \cdot a_2}{2^{k_1} \cdot 2^{k_2}}\right) = (a_1 \cdot a_2, k_1 + k_2)$$

$$\theta(q_1) \cdot \theta(q_2) = (a_1, k_1) \cdot (a_2, k_2) = (a_1 \cdot a_2, k_1 + k_2)$$

$$\text{so, } \theta(q_1 \cdot q_2) = \theta(q_1) \cdot \theta(q_2)$$

**Claim:**  $\theta$  is a function from  $U$  to  $\mathbb{F}$

**Proof:** We need to show that if  $q_1 = q_2$  then  $\theta(q_1) \equiv \theta(q_2)$

$$\begin{aligned} q_1 &= q_2 \\ \frac{a_1}{b_1} &= \frac{a_2}{b_2} \\ a_1 \cdot b_2 &= a_2 \cdot b_1 \\ \ell \cdot 2^{r_1} \cdot 2^{k_2} &= s \cdot 2^{r_2} \cdot 2^{k_1} \end{aligned}$$

because we can write:  $a_1 = \ell \cdot 2^{r_1}$  and  $a_2 = s \cdot 2^{r_2}$ .

$$\ell \cdot 2^{r_1+k_2} = s \cdot 2^{r_2+k_1}$$

so this implies  $\ell = s$  and  $r_1 + k_2 = r_2 + k_1$ . To see why this is true first assume both sides are greater than one, so by fundamental theorem of arithmetic we can write them as a product of distinct primes. Now  $\ell$  and  $s$  are numbers such that they contain all the other primes except 2.

$$\ell \cdot 2^{r_1+k_2} = s \cdot 2^{r_2+k_1}$$

means that on both sides the primes should be the same, and they should have the same powers. Since  $\ell$  and  $s$  do not contain the prime 2, so therefore  $r_1 + k_2 = r_2 + k_1$  as it's the power of 2.  $\ell = s$  as it contains all the other primes except 2. Also knowing that the powers of 2 on both sides are equal trivially implies  $\ell = s$ . Now if both sides are equal to 1, then  $\ell = s = 1$  and  $r_1 + k_2 = r_2 + k_1 = 0$ . If both sides are zero, this means  $a_1$  and  $a_2$  were both zero, so this implies  $\ell = s = 0$  and  $r_1 + k_2 = r_2 + k_1$  since for any given  $k_1$  and  $k_2$  we could choose arbitrary  $r_1$  and  $r_2$  (as we can write  $0 = 0 \cdot 2^r$  where  $r$  is arbitrary).  $\ell = s$  and  $r_1 + k_2 = r_2 + k_1$  naturally means  $\ell = s \pmod{p}$  and  $r_1 + k_2 = r_2 + k_1 \pmod{p}$  which implies  $\theta(q_1) \equiv \theta(q_2)$  (see definition of the new equivalence relation above) .

**Claim:** If  $p > \max\{2m \cdot 2^{2N_a+2N_b}, 2N_a + 4N_b + \log_2 m\}$  then  $\theta$  is 1-1 function.

**Proof:** We need to prove that if  $\theta(q_1) \equiv \theta(q_2)$  then  $q_1 = q_2$ . Suppose for the sake of contradiction that:

$$\begin{aligned} q_1 &\neq q_2 \\ \frac{a_1}{b_1} &\neq \frac{a_2}{b_2} \\ a_1 \cdot b_2 &\neq a_2 \cdot b_1 \\ \ell \cdot 2^{r_1+k_2} &\neq s \cdot 2^{r_2+k_1} \end{aligned}$$

then either  $\ell \neq s$  or  $r_1 + k_2 \neq r_2 + k_1$

Suppose  $\ell \neq s$ .  $\theta(q_1) \equiv \theta(q_2)$  means that  $\ell = s \pmod{p}$  and  $r_1 + k_2 = r_2 + k_1 \pmod{p}$ . Now  $\ell \neq s$  implies that  $\ell - s = hp$  where  $h$  is an integer other than zero (as  $\ell = s \pmod{p}$ ). So, it follows:

$$\begin{aligned} |\ell - s| &\geq p \\ |\ell| + |s| &\geq p \end{aligned}$$

$|\ell| \leq |\ell \cdot 2^{r_1}| \leq |a_1| \leq m \cdot 2^{2N_a+2N_b}$  where the last inequality uses the bound on the numerator from Claim B.1. Similarly,  $|s| \leq |s \cdot 2^{r_2}| \leq |a_2| \leq m \cdot 2^{2N_a+2N_b}$ . Therefore, it follows:

$$2m \cdot 2^{2N_a+2N_b} \geq p \quad (1)$$

which results in a contradiction as  $p > \max\{2m \cdot 2^{2N_a+2N_b}, 2N_a + 4N_b + \log_2 m\}$   
now suppose  $r_1 + k_2 \neq r_2 + k_1 \pmod{p}$ . We know  $r_1 + k_2 = r_2 + k_1 \pmod{p}$ . Hence, it follows that:

$$|(r_1 + k_2) - (r_2 + k_1)| \geq p$$

$$|(r_1 - r_2) - (k_1 - k_2)| \geq p$$

$$|r_1 - r_2| + |k_1 - k_2| \geq p$$

$|2^{r_1}| \leq |\ell \cdot 2^{r_1}| \leq |a_1| \leq 2^{2N_a+2N_b+\log_2 m}$ . This implies  $r_1 \leq 2N_a + 2N_b + \log_2 m$ . Similarly,  $r_2 \leq 2N_a + 2N_b + \log_2 m$ . Hence,  $|r_1 - r_2| \leq 2N_a + 2N_b + \log_2 m$ . Now,  $b_1 = 2^{k_1} \leq 2^{2N_b}$  (follows from the denominator bound in Claim B.1). This implies  $k_1 \leq 2N_b$  and  $k_2 \leq 2N_b$ ,  $|k_1 - k_2| \leq 2N_b$  then immediately follows. Using the above results:

$$2N_a + 2N_b + \log_2 m + 2N_b \geq p$$

$$2N_a + 4N_b + \log_2 m \geq p \quad (2)$$

The above leads to a contradiction as  $p > \max\{2m \cdot 2^{2N_a+2N_b}, 2N_a + 4N_b + \log_2 m\}$ , so this means  $\theta$  is a 1-1 function.

Definition B.1, Claim B.3 and Claim B.4 are also applicable with the newer representation. Below are the arguments which justify this:

**Definition B.1:** The canonical form in the new field would be very similar to the canonical form in  $\mathbb{Q}/p$ . An element  $(a, b) \in \theta(U)$  is a canonical form of its equivalence class if  $a \in [0, 2^{N_a}] \cup [p - 2^{N_a}, p)$  and  $b \in \{1, 2, 3, \dots, N_b\}$ . Let  $(e_a, e_b)$  be the canonical form of  $e \in \theta(U)$ , we define  $\theta^{-1}$  as follows:

$$\begin{aligned} \theta^{-1} : \theta(U) &\rightarrow U \\ e &\mapsto \begin{cases} e_a/2^{e_b} & \text{if } 0 \leq e_a \leq 2^{N_a} \\ (e_a - p)/2^{e_b} & \text{if } p - 2^{N_a} \leq e_a < p \end{cases} \end{aligned}$$

**Claim B.3:**  $\theta^{-1}$  is well-defined

Proof: For  $e \in \theta(U)$ , let  $e = (a, b) \sim (c, d)$ , where  $(a, b)$  and  $(c, d)$  are both canonical forms. We wish to show that  $\theta^{-1}((a, b)) = \theta^{-1}((c, d))$ .

We have  $\theta^{-1}((a, b)) \in U$  and  $\theta^{-1}((c, d)) \in U$ , by definition of  $\theta^{-1}$  and  $U$ . Also we have  $\theta(\theta^{-1}((a, b))) \sim (a, b)$ , as follows. If  $a \in [0, 2^{N_a}]$ , then  $\theta^{-1}((a, b)) = a/2^b$  and  $\theta(a/2^b) = (a, b)$ . If  $a \in [p - 2^{N_a}, p)$ , then  $\theta^{-1}((a, b)) = (a - p)/2^b$  and  $\theta((a - p)/2^b) = (a - p \bmod p, b) \sim (a, b)$ . Likewise,  $\theta(\theta^{-1}((c, d))) \sim (c, d)$ . Now let  $u_1 = \theta^{-1}((a, b))$  and  $u_2 = \theta^{-1}((c, d))$ . Assume for the sake of contradiction that  $u_1 \neq u_2$ ; then  $\theta((u_1)) \sim \theta((u_2))$ , by 1-1 property of the  $\theta$  mapping (as proved above). Thus  $(a, b) \sim \theta(\theta^{-1}((a, b))) \sim \theta(\theta^{-1}((c, d))) \sim (c, d)$ , a contradiction

**Claim B.4:** An element in  $\theta(U)$  cannot have two canonical representations  $(a, b)$  and  $(c, d)$  with  $a \in [0, 2^{N_a}]$  and  $c \in [p - 2^{N_a}, p)$ .

Proof: Take  $(a, b) \sim (c, d)$  where  $a \in [0, 2^{N_a}]$  and  $c \in [p - 2^{N_a}, p)$  where  $b, d \geq 0$ . Because  $\theta^{-1}$  is a function (claim B.3), so  $\theta^{-1}((a, b)) = \theta^{-1}((c, d))$ . However  $\theta^{-1}((a, b)) = a/2^b \geq 0$  and

$\theta^{-1}((c, d)) = (c - p)/2^d < 0$ , which is a contradiction.

*Implementation details:*

The computation in new field is isomorphic to computation in  $\mathbb{Z}/p$ , via the following map:

$$f : \mathbb{F} \rightarrow \mathbb{Z}/p$$

$$(a, b) \mapsto a2^{-b}$$

$f$  preserves addition and multiplication rules:

$$f((a, b)) \cdot f((c, d)) = a2^{-b} \cdot c2^{-d} = ac \cdot 2^{-b-d}$$

$$f((a, b) \cdot (c, d)) = f((ac, b + d)) = ac \cdot 2^{-b-d}$$

$$\text{Hence, } f((a, b) \cdot (c, d)) = f((a, b)) \cdot f((c, d))$$

Similarly, for addition:

$$f((a, b)) + f((c, d)) = a2^{-b} + c2^{-d}$$

$$f((a, b) + (c, d)) = f((a2^d + c2^b, b + d)) = (a2^d + c2^b) \cdot 2^{-b-d} = a2^{-b} + c2^{-d}$$

$$\text{Hence } f((a, b) + (c, d)) = f((a, b)) + f((c, d))$$

**Claim:**  $f$  is a function from  $\mathbb{F}$  to  $\mathbb{Z}/p$

**Proof:** we need to prove that if  $(a, b) \sim (c, d)$  then  $f((a, b)) = f((c, d))$

assume that  $(a, b) \sim (c, d)$ , where  $a = \ell \cdot 2^{r_1}$  and  $c = s \cdot 2^{r_2}$  then:

$$\ell \equiv s \pmod{p}$$

$$r_1 + d \equiv r_2 + b \pmod{p}$$

now  $\ell \equiv s \pmod{p}$  implies  $\ell = s$ , because  $\ell \neq s$  means  $|\ell - s| \geq p$  which as shown in (1) leads to a contradiction. So,  $\ell = s$

Similarly,  $r_1 + d \equiv r_2 + b \pmod{p}$  implies  $r_1 + d = r_2 + b$ , because  $r_1 + d \neq r_2 + b$  means  $|r_1 + d - (r_2 + b)| \geq p$  which as shown in (2) leads to a contradiction. So,  $r_1 + d = r_2 + b$ .

Furthermore,  $r_1 + d = r_2 + b$  implies  $2^{r_1+d} = 2^{r_2+b}$

$\ell = s$  and  $2^{r_1+d} = 2^{r_2+b}$ , then leads to  $\ell \cdot 2^{r_1+d} = s \cdot 2^{r_2+b}$ , or  $\ell \cdot 2^{r_1+d} = s \cdot 2^{r_2+b} \pmod{p}$ .

$$\ell \cdot 2^{r_1+d} = s \cdot 2^{r_2+b} \pmod{p}$$

$$a2^d = c2^b \pmod{p}$$

$$a2^{-b} = c2^{-d} \pmod{p}$$

Hence,  $f((a, b)) = f((c, d))$ .

**Claim:**  $f$  is 1-1 from  $\mathbb{F}$  to  $\mathbb{Z}/p$  if  $p > 2m \cdot 2^{2N_a+4N_b}$

**Proof:** we need to prove that if  $f((a, b)) = f((c, d))$  then  $(a, b) \sim (c, d)$

$$f((a, b)) = f((c, d))$$

$$a2^{-b} \equiv c2^{-d} \pmod{p}$$

$$a2^d \equiv c2^b \pmod{p}$$

$a2^d \equiv c2^b \pmod{p}$  implies  $a2^d = c2^b$  because  $a2^d \neq c2^b$  results in a contradiction as shown below:

$$|a2^d - c2^b| \geq p$$

$$|a2^d| + |c2^b| \geq p$$

$|a2^d| \leq |a| \cdot 2^d \leq m \cdot 2^{2N_a+4N_b} (as \mid a \leq m \cdot 2^{2N_a+2N_b} \text{ and } 2^d \leq 2^{2N_b})$ . Similarly,  $|c2^b| \leq |c| \cdot 2^b \leq m \cdot 2^{2N_a+4N_b}$ . Hence, it follows:

$$|a2^d| + |c2^b| \leq 2m \cdot 2^{2N_a+4N_b}$$

$$2m \cdot 2^{2N_a+4N_b} \geq p$$

The above inequality results in a contradiction given  $p > 2m \cdot 2^{2N_a+4N_b}$  writing  $a = \ell \cdot 2^{r_1}$  and  $c = s \cdot 2^{r_2}$  and substituting then gives:

$$\ell 2^{r_1+d} = s 2^{r_2+b}$$

which implies  $\ell = s$  and  $r_1 + d = r_2 + b$ , or  $\ell \equiv s \pmod{p}$  and  $r_1 + d \equiv r_2 + b \pmod{p}$ . So,  $(a, b) \sim (c, d)$ . So, computation in the field  $\mathbb{F}$  is isomorphic to computation in the field  $\mathbb{Z}/p$ .

**Definition B.2(GINGER-Q protocol):** Let  $\Psi$  be a computation over  $\mathbb{F}$ , and let  $\Psi'$  be the same computation, expressed over  $\mathbb{Z}/p$ . The GINGER-Q protocol for verifying  $\Psi$  is defined as follows:

1.  $V \rightarrow P$ : a vector  $x$ , over the domain  $\mathbb{F}$
2.  $P \rightarrow V$ :  $y = \Psi(x)$ .
3.  $P \rightarrow V$ :  $x'$  and  $y'$ .  $P$  obtains  $x', y'$  (which are vectors in  $\mathbb{Z}/p$ ) by applying  $f$  elementwise to  $x$  and  $y$ .
4.  $V$  checks that for all  $(a, b) \in \{x \cup y\}$  and the corresponding element  $c \in \{x' \cup y'\}$ ,  $c2^b \equiv a \pmod{p}$ . This confirms that  $P$  has applied  $f$  correctly. If the check fails,  $V$  rejects.
5.  $V$  engages  $P$  using the existing GINGER implementation, to verify that  $y' = \Psi'(x')$ .

Next I describe simple modifications to appendix C(C.3 and C.4).

**Claim C.3**  $\theta(x_1) - \theta(x_2) \in \theta(S)$  if and only if the numerator in the canonical representation of  $\theta(x_1) - \theta(x_2)$  is contained in  $[p - 2^{N_a}, p)$ .

**Proof:** We will use the definition of  $\theta^{-1}$  in the previous appendix. Let  $e = \theta(x_1) - \theta(x_2)$ . If  $e \in \theta(S)$ , then  $\theta^{-1}(e) = a/2^b$ , where  $a \in [-2^{N_a}, 0)$  and  $2^b \in \{1, 2, 2^2, \dots, 2^{N_b}\}$ . Thus,  $\theta(a/2^b) = (p + a, b)$ , where  $p + a \in [p - 2^{N_a}, p)$ , and  $\theta(a/2^b) = \theta(\theta^{-1}(e)) \sim e$ , so  $e$  has a canonical representation of the required form. On the other hand, if  $e \sim (a, b)$ , where  $a \in [p - 2^{N_a}, p)$ , then  $\theta^{-1}(e) = (a - p)/2^b \in S$ , so  $e \sim \theta(\theta^{-1}(e)) \in \theta(S)$ .

We instantiate step C3 with the following constraints  $\mathcal{C}_<$ :

$$\mathcal{C}_< = \left\{ \begin{array}{ll} A_0((1, 0) - A_0) & = (0, 1), \\ A_1((2, 0) - A_1) & = (0, 1), \\ \vdots & \vdots \\ A_{N_a-1}((2^{N_a-1}, 0) - A_{N_a-1}) & = (0, 1), \\ A - (p - 2^{N_a}, 0) - \sum_{i=0}^{N_a-1} A_i & = (0, 1), \\ B_0((1, 0) - B_0) & = (0, 1), \\ B_1((1, 0) - B_1) & = (0, 1), \\ \vdots & \vdots \\ B_{N_b}((1, 0) - B_{N_b}) & = (0, 1), \\ \sum_{i=0}^{N_b} B_i - (1, 0) & = (0, 1), \\ B - \sum_{i=0}^{N_b} B_i \cdot (1, i) & = (0, 1), \\ \theta(X_1) - \theta(X_2) - A \cdot B & = (0, 1) \end{array} \right\}$$

**Lemma C.4 :**  $\mathcal{C}_<$  is satisfiable if and only if the numerator in the canonical representation of  $\theta(x_1) - \theta(x_2)$  is contained in  $[p - 2^{N_a}, p)$ .

**Proof:** Assume that  $X_3 = \theta(x_1) - \theta(x_2)$  has the required form  $(a, b)$ . We have  $b \in \{0, 1, 2, \dots, N_b\}$  and  $a \in [p - 2^{N_a}, p)$ . Now, take  $B_{\mathbf{b}} = (1, 0)$  and all other  $B_j = (0, 1)$ ; this satisfies all of the  $B_i$  constraints, including  $\sum_{i=0}^{N_b} B_i - (1, 0) = (0, 1)$ , which requires that exactly one  $B_i$  be equal to  $(1, 0)$ . For  $B$ , take  $B = (1, b)$ , to satisfy  $B - \sum_{i=0}^{N_b} B_i \cdot (1, i) = (0, 1)$ .

Now, let  $a' = a - (p - 2^{N_a})$ . The binary representation of  $a'$  has bits  $z_0, z_1, \dots, z_{N_a-1}$ . Set  $A_i = (z_i, 0)(2^i, 0)$  for  $i \in \{0, 1, \dots, N_a - 1\}$ . This will satisfy all of the individual  $A_i$  constraints. And, since  $\sum_{i=0}^{N_a-1} A_i = (a', 0)$ , we can take  $A = (a, 0)$  to satisfy  $A - (p - 2^{N_a}, 0) - \sum_{i=0}^{N_a-1} A_i = (0, 1)$ . The remaining constraint is the last one in the list. It is satisfiable because we took  $B = (1, b)$  and  $A = (a, 0)$ , giving  $X_3 - (a, 0) \cdot (1, b) = (0, 1)$ .

For the other direction, if the constraints are satisfiable, then  $X_3 = \theta(x_1) - \theta(x_2)$  can be written as  $(a, 0)(1, b)$ , where  $b \in \{1, 2, \dots, N_b\}$  and where  $a = p - 2^{N_a} + \sum_{i=0}^{N_a-1} z_i 2^i$ , for  $z_i \in \{0, 1\}$ . This implies that  $a \in [p - 2^{N_a}, p)$ .